\documentclass[russian]{article}
\usepackage[T1]{fontenc}
\usepackage[utf8]{inputenc}
\usepackage{amsmath,amssymb,esint,babel}
\makeatletter
\makeatother
\pagestyle{myheadings}
\markright{Александров А., 3372}

\begin{document}
\section*{1.1}
\paragraph*{а}
$(xy' - 1) \ln x = 2y$

$(x \frac{dy}{dx} - 1) \ln x = 2y$

$\frac{dy}{dx} = \frac{2}{x \ln x} y + \frac{1}{x}$

$\begin{cases}
y(x) = C(x) e^{\int \frac{2}{x \ln x} dx} \\
\frac{dC}{dx} = \frac{1}{x} e^{-\int \frac{2}{x \ln x} dx}
\end{cases}$

$\int \frac{2}{x \ln x} dx = 2 \ln \ln x + c_0$

$\begin{cases}
y(x) = C(x) e^{2 \ln \ln x + c_0} = C(x) e^{c_0} \ln ^2 x\\
\frac{dC}{dx} = \frac{1}{x} e^{-2 \ln \ln x - c_0} = \frac{1}{e^{c_0} x \ln ^2 x}
\end{cases}$

$C(x) = \int \frac{1}{e^{c_0} x \ln ^2 x} dx + c_1 = - \frac{1}{e^{c_0} \ln x} + c_1$

$y(x) = C(x) e^{c_0} \ln ^2 x = -\ln x + c_1 e^{c_0} \ln ^2 x = c \ln ^2 x - \ln x$

\end{document}